closure

Foundation/Modal/Kripke/Basic.lean
@@ -18,12 +18,6 @@ instance : CoeSort Frame (Type) := ⟨Frame.World⟩
 instance : CoeFun Frame (λ F => F.World → F.World → Prop) := ⟨Frame.Rel⟩
 instance {F : Frame} : Nonempty F.World := F.world_nonempty
 
-abbrev Frame.Rel' {F : Frame} (x y : F.World) := F.Rel x y
-infix:45 " ≺ " => Frame.Rel'
-
-protected abbrev Frame.RelItr' {F : Frame} (n : ℕ) := F.Rel.iterate n
-notation x:45 " ≺^[" n "] " y:46 => Frame.RelItr' n x y
-
 
 structure FiniteFrame extends Frame where
   [world_finite : Finite World]
@@ -34,12 +28,110 @@ instance {F : FiniteFrame} : Finite F.World := F.world_finite
 def Frame.toFinite (F : Frame) [Finite F.World] : FiniteFrame := ⟨F⟩
 
 
+namespace Frame
+
+open Relation
+
+variable {F : Frame} {x y : F.World}
+
+abbrev Rel' (x y : F.World) := F.Rel x y
+infix:45 " ≺ " => Frame.Rel'
+
+abbrev RelItr' (n : ℕ) := F.Rel.iterate n
+notation x:45 " ≺^[" n "] " y:46 => Frame.RelItr' n x y
+
+abbrev RelReflTransGen : _root_.Rel F.World F.World := ReflTransGen (· ≺ ·)
+infix:45 " ≺^* " => Frame.RelReflTransGen
+
+namespace RelReflTransGen
+
+lemma single (hxy : x ≺ y) : x ≺^* y := ReflTransGen.single hxy
+
+@[simp]
+protected lemma reflexive : Reflexive F.RelReflTransGen := Relation.reflexive_reflTransGen
+
+@[simp]
+lemma refl {x : F.World} : x ≺^* x := RelReflTransGen.reflexive x
+
+@[simp]
+protected lemma transitive : Transitive F.RelReflTransGen := Relation.transitive_reflTransGen
+
+protected lemma symmetric : Symmetric F.Rel → Symmetric F.RelReflTransGen := ReflTransGen.symmetric
+
+protected lemma exists_itr : x ≺^* y ↔ ∃ n, F.Rel.iterate n x y := ReflTransGen.exists_iterate
+
+end RelReflTransGen
+
+abbrev TransitiveReflexiveClosure (F : Frame) : Frame := ⟨F.World, (· ≺^* ·)⟩
+postfix:95 "^*" => Frame.TransitiveReflexiveClosure
+
+
+abbrev RelTransGen {F : Frame} : _root_.Rel F.World F.World := TransGen (· ≺ ·)
+infix:45 " ≺^+ " => Frame.RelTransGen
+
+namespace RelTransGen
+
+protected lemma single (hxy : x ≺ y) : x ≺^+ y := TransGen.single hxy
+
+@[simp]
+protected lemma transitive : Transitive F.RelTransGen := λ _ _ _ => TransGen.trans
+
+protected lemma symmetric (hSymm : Symmetric F.Rel) : Symmetric F.RelTransGen := by
+  intro x y rxy;
+  induction rxy with
+  | single h => exact TransGen.single $ hSymm h;
+  | tail _ hyz ih => exact TransGen.trans (TransGen.single $ hSymm hyz) ih
+
+lemma exists_itr : x ≺^+ y ↔ ∃ n > 0, F.Rel.iterate n x y := TransGen.exists_iterate
+
+end RelTransGen
+
+abbrev TransitiveClosure (F : Frame) : Frame := ⟨F.World, (· ≺^+ ·)⟩
+postfix:95 "^+" => Frame.TransitiveClosure
+
+
+abbrev RelReflGen : _root_.Rel F.World F.World := ReflGen (· ≺ ·)
+infix:45 " ≺^= " => Frame.RelReflGen
+
+def ReflexiveClosure (F : Frame) : Frame := ⟨F.World, (· ≺^= ·)⟩
+postfix:95 "^=" => Frame.ReflexiveClosure
+
+
+abbrev RelIrreflGen : _root_.Rel F.World F.World := IrreflGen (· ≺ ·)
+scoped infix:45 " ≺^≠ " => Frame.RelIrreflGen
+
+def IrreflexiveClosure (F : Frame) : Frame := ⟨F.World, (· ≺^≠ ·)⟩
+postfix:95 "^≠" => Frame.IrreflexiveClosure
+
+namespace IrreflexiveClosure
+
+@[simp]
+lemma rel_irreflexive : Irreflexive (F^≠.Rel) := by
+  simp [Irreflexive, Frame.RelIrreflGen, IrreflGen, Frame.IrreflexiveClosure]
+
+end IrreflexiveClosure
+
+end Frame
+
+
+instance {F : FiniteFrame} : Finite (F.toFrame^=).World := by simp [Frame.ReflexiveClosure];
+
+abbrev FiniteFrame.ReflexiveClosure (F : FiniteFrame) : FiniteFrame := ⟨F.toFrame^=⟩
+postfix:95 "^=" => FiniteFrame.ReflexiveClosure
+
+instance {F : FiniteFrame} : Finite (F.toFrame^≠).World := by simp [Frame.IrreflexiveClosure]
+
+abbrev FiniteFrame.IrreflexiveClosure (F : FiniteFrame) : FiniteFrame := ⟨F.toFrame^≠⟩
+postfix:95 "^≠" => FiniteFrame.IrreflexiveClosure
+
+
 section
 
 abbrev whitepoint : FiniteFrame := ⟨Unit, λ _ _ => True⟩
 abbrev blackpoint : FiniteFrame := ⟨Unit, λ _ _ => False⟩
 
 end
+
 
 abbrev FrameClass := Set (Frame)
 
